Finish some more of the heapspec reasoning
The wal_heap_h mapsto facts seem important for reconstructing the txn
system, but they get modified in some way. The current recovery proof
doesn't track them at all, but the infrastructure is there to do so once
we figure out what txn needs.

src/program_proof/wal/heapspec.v
@@ -164,6 +164,176 @@ Proof.
     rewrite Nat.min_l //.
 Qed.
 
+Lemma wal_heap_inv_addr_crash ls k x crash_txn :
+  ls.(log_state.installed_lb) ≤ crash_txn →
+  let ls' := (set log_state.txns (take (S crash_txn)) ls)
+                <| log_state.durable_lb := crash_txn |> in
+  wal_heap_inv_addr ls k x -∗
+  wal_heap_inv_addr ls' k x.
+Proof.
+  intros Hbound.
+  rewrite /wal_heap_inv_addr //=.
+  iPureIntro.
+  intros [? Hinstalled].
+  split; [done|].
+  destruct x as [installed_block blocks_since_install].
+  destruct Hinstalled as (txn_id & ?&?&?).
+  exists txn_id.
+  split_and!; [done | | ].
+  - rewrite /disk_at_txn_id /=.
+    rewrite -> take_take, Nat.min_l by lia.
+    assumption.
+  - rewrite /updates_since /=.
+    admit. (* TODO(tej): not true, blocks since install change when we take a
+    prefix of transactions (x won't be the same) *)
+Abort.
+
+(* TODO(tej): drop_end is a useless notion; I originally thought the
+blocks_since_install could be computed by removing the right number of blocks
+from the old blocks_since_install, but this is the filtered set of updates to a
+particular address. We need to know the existential txn_id being used to say how
+that list gets prefixed on crash. *)
+
+Definition drop_end {A} (n: nat) (l: list A) :=
+  take (length l - n) l.
+
+Lemma drop_end_to_take {A} n (l: list A) :
+  (n ≤ length l)%nat →
+  drop_end (length l - n) l = take n l.
+Proof.
+  intros.
+  rewrite /drop_end.
+  auto with f_equal lia.
+Qed.
+
+Lemma drop_drop_end {A} n m (l: list A) :
+  drop n (drop_end m l) = drop_end m (drop n l).
+Proof.
+  rewrite /drop_end.
+  rewrite take_drop_commute.
+  rewrite drop_length.
+  destruct (decide (n + m ≤ length l)).
+  - auto with f_equal lia.
+  - rewrite !drop_ge //; len.
+Qed.
+
+Definition heap_block_blocks_since_install (hb: heap_block) :=
+  let 'HB _ blocks_since_install := hb in blocks_since_install.
+
+Instance list_fmap_respects_prefix_of {A B} (f: A → B) : Proper (prefix ==> prefix) (fmap f).
+Proof.
+  intros l1 l2 [l' ->].
+  eexists.
+  rewrite fmap_app //.
+Qed.
+
+Instance list_filter_respects_prefix_of {A} (f: A → Prop) `{!∀ x, Decision (f x)} :
+  Proper (prefix ==> prefix) (filter f).
+Proof.
+  intros l1 l2 [l' ->].
+  eexists.
+  rewrite filter_app //.
+Qed.
+
+Instance concat_respects_prefix {A} : Proper (prefix ==> prefix) (concat (A:=A)).
+Proof.
+  intros l1 l2 [l' ->].
+  eexists.
+  rewrite concat_app //.
+Qed.
+
+Lemma take_prefix {A} (l1 l2: list A) n :
+  l1 `prefix_of` l2 →
+  take n l1 `prefix_of` l2.
+Proof.
+  intros [l' ->].
+  exists (drop n l1 ++ l').
+  rewrite app_assoc.
+  rewrite take_drop //.
+Qed.
+
+Lemma wal_heap_inv_addr_crash ls a b crash_txn :
+  ls.(log_state.installed_lb) ≤ crash_txn < length ls.(log_state.txns) →
+  let ls' := (set log_state.txns (take (S crash_txn)) ls)
+                <| log_state.durable_lb := crash_txn |> in
+  wal_heap_inv_addr ls a b -∗
+  ∃ b', ⌜heap_block_blocks_since_install b' `prefix_of` heap_block_blocks_since_install b⌝ ∗
+         wal_heap_inv_addr ls' a b'.
+Proof.
+  intros Hbound.
+  rewrite /wal_heap_inv_addr //=.
+  iPureIntro.
+  intros [? Hinstalled].
+  destruct b as [installed_block blocks_since_install].
+  destruct Hinstalled as (txn_id & ?&?&?).
+  eexists (HB installed_block _).
+  split_and!; [ | done | ].
+  2: {
+    exists txn_id.
+    split_and!; [done | | ].
+    - rewrite /disk_at_txn_id /=.
+      rewrite -> take_take, Nat.min_l by lia.
+      assumption.
+    - rewrite //=.
+  }
+  simpl.
+  rewrite /updates_since /= in H2 |- *.
+  rewrite skipn_firstn_comm.
+  rewrite -H2.
+  rewrite /updates_for_addr.
+  f_equiv.
+  f_equiv.
+  rewrite /txn_upds.
+  f_equiv.
+  f_equiv.
+  apply take_prefix.
+  reflexivity.
+Qed.
+
+Lemma wal_heap_gh_crash crash_txn (gh: gmap u64 heap_block) ls :
+  ls.(log_state.installed_lb) ≤ crash_txn < length ls.(log_state.txns) →
+  let ls' := (set log_state.txns (take (S crash_txn)) ls)
+                <| log_state.durable_lb := crash_txn |> in
+  ([∗ map] a↦b ∈ gh, wal_heap_inv_addr ls a b) -∗
+  |==> ∃ (γ': gen_heapG u64 heap_block Σ) gh',
+      ⌜dom (gset _) gh' = dom (gset _) gh⌝ ∗
+      gen_heap_ctx (hG:=γ') gh' ∗
+      (* TODO: something has been lost along the way about how these values
+      relate to the old ones; probably the exchanger is the only thing that can
+      contain that information *)
+      [∗ map] a↦b ∈ gh', wal_heap_inv_addr ls' a b.
+Proof using walheapG0.
+  intros Hbound.
+  cbn zeta.
+  iIntros "#Hinv".
+  iInduction gh as [|a b gh] "IH" using map_ind.
+  - iMod (gen_heap_init (∅ : gmap u64 heap_block)) as (γwal_heap_h) "Hgh'".
+    iModIntro.
+    iExists _, ∅.
+    rewrite dom_empty_L.
+    rewrite big_sepM_empty.
+    by iFrame.
+  - rewrite big_sepM_insert //.
+    iDestruct "Hinv" as "[Ha Hinv]".
+    iMod ("IH" with "[//]") as (γ' gh' Hdom) "[Hctx #Hinv']".
+    iExists γ'.
+    iDestruct (wal_heap_inv_addr_crash _ _ _ crash_txn with "Ha") as (b' Hprefix) "Ha'".
+    { lia. }
+    assert (gh' !! a = None).
+    { apply not_elem_of_dom.
+      rewrite Hdom.
+      apply not_elem_of_dom; done. }
+    iMod (gen_heap_alloc _ a b' with "Hctx") as "[Hctx Hmapsto]"; first by auto.
+    (* TODO: this is where we're not collecting the mapsto facts *)
+    iModIntro.
+    iExists (<[a:=b']> gh').
+    iFrame.
+    rewrite !dom_insert_L //.
+    iSplit; first by (iPureIntro; congruence).
+    rewrite big_sepM_insert //.
+    iFrame "#".
+Qed.
+
 Lemma wal_heap_inv_crash_transform γ ls ls' :
   relation.denote log_crash ls ls' () →
   wal_heap_inv γ ls -∗
@@ -195,6 +365,13 @@ Proof.
                     subst ls'; rename ls'' into ls';
                     fold ls'
   end. simpl.
+  (* TODO: note that this loses the old map, which makes it impossible to use
+  those resources to write an exchanger for wal_heap_h mapsto facts in the old
+  generation (don't know if those are useful) *)
+  iMod (wal_heap_gh_crash crash_txn with "Hgh") as
+      (γwal_heap_h gh' Hdom) "[Hctx' Hgh'] {Hctx}".
+  { destruct Hwf.
+    lia. }
   iMod (ghost_var_alloc (ls.(log_state.d), ls'.(log_state.txns)))
     as (wal_heap_txns_name) "[Htxns' Htxns2]".
   iMod (ghost_var_alloc (list_to_async (take (S crash_txn) (possible crash_heaps))))
@@ -202,7 +379,8 @@ Proof.
   iMod (mnat_alloc crash_txn) as (wal_heap_durable_lb_name) "[Hcrash_heaps_lb' Hcrash_heaps_lb_lb]".
 
   iModIntro.
-  iExists (γ <| wal_heap_txns := wal_heap_txns_name |>
+  iExists (γ <| wal_heap_h := γwal_heap_h |>
+             <| wal_heap_txns := wal_heap_txns_name |>
              <| wal_heap_crash_heaps := wal_heap_crash_heaps_name |>
              <| wal_heap_durable_lb := wal_heap_durable_lb_name |>).
   rewrite /wal_heap_inv /=.
@@ -212,14 +390,8 @@ Proof.
   { iExists _; iFrame.
     by rewrite -> take_length_le by lia. }
   iExists _, _; iFrame "#∗%".
-  iSplit.
-  { iApply (big_sepM_mono with "Hgh").
-    intros ?? _.
-    rewrite /wal_heap_inv_addr /ls' //=.
-    admit. (* seems about right, using wal_wf to show crash_txn is above installed_lb *) }
   iApply (wal_heap_inv_crashes_crash with "Hcrash_heaps"); auto.
-  all: fail "goals remaining".
-Admitted.
+Qed.
 
 Definition locked_wh_disk (lwh : locked_walheap) : disk :=
   apply_upds (txn_upds lwh.(locked_wh_σtxns)) lwh.(locked_wh_σd).
